ZiskFv/Compliance/MainTransition.lean
@@ -101,6 +101,7 @@ theorem AcceptedZiskTrace.mainTransition_to_next_pc
   change ZiskFv.AirsClean.Main.pcHandshakeTransition transitionIndex.val
     (trace.mainTable.previousEnvironment transitionIndex)
     (trace.mainTable.environmentAt transitionIndex) at h_trans
+  have h_trans_pc := h_trans.1
   have h_transition : ZiskFv.AirsClean.Main.pcHandshakeBetween
       ((ZiskFv.AirsClean.Main.componentWithRomMemAndOpBus
           trace.programLength trace.program).rowInput
@@ -109,7 +110,7 @@ theorem AcceptedZiskTrace.mainTransition_to_next_pc
           trace.programLength trace.program).rowInput
         (trace.mainTable.environmentAt transitionIndex)) := by
     simpa only [ZiskFv.AirsClean.Main.pcHandshakeTransition, Air.Flat.Component.rowInput,
-      Air.Flat.Component.rowInputVar, eval_varFromOffset_valueFromOffset] using h_trans
+      Air.Flat.Component.rowInputVar, eval_varFromOffset_valueFromOffset] using h_trans_pc
   have h_previous := rowInputPrevious_eq_mainTableRowAtOrZero trace.program trace.mainTable
     transitionIndex (by simp [transitionIndex])
   have h_current := rowInputAt_eq_mainTableRowAtOrZero trace.program trace.mainTable
